examples/mutsum/MutFImp0proof.v
@@ -41,7 +41,8 @@ Section SIMMODSEM.
       (<<TGT: mrps_tgt0 = (ε, tt↑)>>)
   .
   
-  Theorem correct: ModSemPair.sim MutF0.FSem MutFImp.FSem.
+  Theorem correct:
+    forall ge, ModSemPair.sim MutF0.FSem (MutFImp.FSem ge).
   Proof.
     econstructor 1 with (wf:=wf); et; ss.
     econs; ss. init. unfold cfun.
